Move bounded_u8 to Int. Prepare for sums

examples/miniparse/MiniParse.Spec.TEnum.fst
@@ -6,9 +6,6 @@ include MiniParse.Spec.Int
 module T = FStar.Tactics
 module U8 = FStar.UInt8
 
-inline_for_extraction
-let mk_u8 (n: nat { n < 256 } ) : Tot U8.t = U8.uint_to_t n
-
 let rec mk_tenum_branches (ty: T.term) (vty: T.term) (v: nat) (accu: list T.branch) (l: list T.name) : T.Tac (list T.branch) =
   match l with
   | [] -> accu
@@ -136,31 +133,6 @@ let invert_function (enum_ty val_ty: T.term) (teq: T.term) (f: T.term) : T.Tac u
     end
   | _ -> T.fail "Not a global variable"
 
-inline_for_extraction
-let bounded_u8 (b: nat) : Tot eqtype = (x: U8.t { U8.v x < b } )
-
-inline_for_extraction
-let bounded_fun (a: Type) (b: nat) : Tot Type =
-  a -> Tot (bounded_u8 b)
-
-inline_for_extraction
-let map_u8_to_bounded_u8
-  (a: Type)
-  (bound: nat)
-  (f: (a -> Tot U8.t))
-  (g: (x: a) -> Tot (squash (U8.v (f x) < bound)))
-  (a' : Type)
-  (bound' : nat)
-  (u1: squash (a == a'))
-  (u2: squash (bound == bound'))
-: Tot (bounded_fun a' bound')
-= fun x ->
-  [@inline_let]
-  let _ = g x in
-  [@inline_let]
-  let y' : bounded_u8 bound = f x in
-  y'
-
 let tenum_bound_nat (t: T.term) : T.Tac nat =
   let c = get_inductive_constructors t in
   List.Tot.length c
@@ -180,51 +152,6 @@ let gen_synth_bounded (t: T.term) : T.Tac unit =
   T.set_guard_policy T.Goal;
   T.exact_guard (gen_synth_bounded' t);
   tconclude ()
-
-let pred_pre
-  (bound: nat { bound > 0 /\ bound <= 256 } )
-  (pred: bounded_u8 bound -> GTot Type0)
-  (x: bounded_u8 (bound - 1))
-: GTot Type0
-= pred (x `U8.add` 1uy)
-
-let pred_large_bound
-  (bound: nat { bound > 256 } )
-  (pred: bounded_u8 bound -> GTot Type0)
-  (x: bounded_u8 (bound - 1))
-: GTot Type0
-= pred (x <: U8.t)
-
-let rec forall_bounded_u8
-  (bound: nat)
-  (pred: (bounded_u8 bound -> GTot Type0))
-: GTot Type0
-= if bound = 0
-  then True
-  else if bound > 256
-  then
-    forall_bounded_u8 (bound - 1) (pred_large_bound bound pred)
-  else
-    pred 0uy /\ forall_bounded_u8 (bound - 1) (pred_pre bound pred)
-
-let rec forall_bounded_u8_elim
-  (bound: nat)
-  (pred: (bounded_u8 bound -> GTot Type0))
-  (x: bounded_u8 bound)
-: Lemma
-  (requires (forall_bounded_u8 bound pred))
-  (ensures (pred x))
-  (decreases bound)
-= if bound = 0
-  then ()
-  else if bound > 256
-  then
-    let x' : bounded_u8 (bound - 1) = x <: U8.t in
-    forall_bounded_u8_elim (bound - 1) (pred_large_bound bound pred) x'
-  else if x = 0uy
-  then ()
-  else
-    forall_bounded_u8_elim (bound - 1) (pred_pre bound pred) (x `U8.sub` 1uy)
 
 let synth_inverse_forall_bounded_u8_pred
   (b: nat)
@@ -315,16 +242,6 @@ let synth_inverse_forall_bounded_u8_solve () : T.Tac unit =
     end else tfail "Goal is not synth_injective"
   | _ -> tfail "Not enough arguments to squash"
   else tfail "Goal is not squash"
-
-inline_for_extraction
-let bounded_u8_eq (b: nat) : Tot (bounded_u8 b -> bounded_u8 b -> Tot bool) =
-  op_Equality
-
-let parse_bounded_u8 (b: nat) : Tot (parser (bounded_u8 b)) =
-  parse_synth
-    (parse_filter parse_u8 (fun x -> U8.v x < b))
-    (fun x -> x <: bounded_u8 b)
-    (fun x -> x)
 
 (* WARNING: the following tactic may leave some VC goals behind *)
 
