examples/miniparse/MiniParse.Impl.Int.fst
@@ -21,3 +21,27 @@ let serialize32_u8 : serializer32 serialize_u8 =
       assert (B.as_seq h' output' `Seq.equal` Seq.create 1 x);
       Some 1ul
     end)
+
+#set-options "--z3rlimit 16"
+
+inline_for_extraction
+let parse32_bounded_u8
+  (b: nat)
+: Tot (parser32 (parse_bounded_u8 b)) =
+  if b >= 256
+  then (fun input len -> parse32_synth parse32_u8 (fun x -> x <: bounded_u8 b) (fun x -> x <: bounded_u8 b) (fun x -> x) () input len)
+  else
+    [@inline_let]
+    let b' = U8.uint_to_t b in
+    parse32_synth
+      (parse32_filter parse32_u8 (fun x -> U8.v x < b) (fun x -> x `U8.lt` b'))
+      (fun x -> x <: bounded_u8 b)
+      (fun x -> x <: bounded_u8 b)
+      (fun x -> x)
+      ()
+
+#reset-options
+
+inline_for_extraction
+let serialize32_bounded_u8 (b: nat) : Tot (serializer32 (serialize_bounded_u8 b)) =
+  fun output len x -> serialize32_u8 output len x
