examples/miniparse/MiniParse.Spec.TSum.fst
@@ -1,0 +1,98 @@
+module MiniParse.Spec.TSum
+include MiniParse.Spec.Combinators
+
+module Seq = FStar.Seq
+
+inline_for_extraction
+let refine_with_tag (#tag_t: Type0) (#data_t: Type0) (tag_of_data: (data_t -> GTot tag_t)) (x: tag_t) : Tot Type0 =
+  (y: data_t { tag_of_data y == x } )
+
+inline_for_extraction
+let synth_tagged_union_data
+  (#tag_t: Type0)
+  (#data_t: Type0)
+  (tag_of_data: (data_t -> GTot tag_t))
+  (tg: tag_t)
+  (x: refine_with_tag tag_of_data tg)
+: Tot data_t
+= x
+
+val parse_tagged_union
+  (#tag_t: Type0)
+  (pt: parser tag_t)
+  (#data_t: Type0)
+  (tag_of_data: (data_t -> GTot tag_t))
+  (p: (t: tag_t) -> Tot (parser (refine_with_tag tag_of_data t)))
+: Tot (parser data_t)
+
+let parse_tagged_union #tag_t pt #data_t tag_of_data p =
+  pt `and_then` (fun (tg: tag_t) ->
+    parse_synth' #(refine_with_tag tag_of_data tg) (p tg) (synth_tagged_union_data tag_of_data tg)
+  )
+
+let bare_serialize_tagged_union
+  (#tag_t: Type0)
+  (#pt: parser tag_t)
+  (st: serializer pt)
+  (#data_t: Type0)
+  (tag_of_data: (data_t -> GTot tag_t))
+  (#p: (t: tag_t) -> Tot (parser (refine_with_tag tag_of_data t)))
+  (s: (t: tag_t) -> Tot (serializer (p t)))
+: Tot (bare_serializer data_t)
+= fun (d: data_t) ->
+  let tg = tag_of_data d in
+  Seq.append (serialize st tg) (serialize (s tg) d)
+
+let bare_serialize_tagged_union_correct
+  (#tag_t: Type0)
+  (#pt: parser tag_t)
+  (st: serializer pt)
+  (#data_t: Type0)
+  (tag_of_data: (data_t -> GTot tag_t))
+  (#p: (t: tag_t) -> Tot (parser (refine_with_tag tag_of_data t)))
+  (s: (t: tag_t) -> Tot (serializer (p t)))
+: Lemma
+  (ensures (serializer_correct (parse_tagged_union pt tag_of_data p) (bare_serialize_tagged_union st tag_of_data s)))
+= (* same proof as nondep_then *)
+  let prf
+    (x: data_t)
+  : Lemma (parse (parse_tagged_union pt tag_of_data p) (bare_serialize_tagged_union st tag_of_data s x) == Some (x, Seq.length (bare_serialize_tagged_union  st tag_of_data s x)))
+  = let t = tag_of_data x in
+    let (u: refine_with_tag tag_of_data t) = x in
+    let v1' = parse pt (bare_serialize_tagged_union st tag_of_data s x) in
+    let v1 = parse pt (serialize st t) in
+    assert (Some? v1);
+    assert (no_lookahead_on (coerce_to_bare_parser _ pt) (serialize st t) (bare_serialize_tagged_union st tag_of_data s x));
+    let (Some (_, len')) = parse pt (serialize st t) in
+    assert (len' == Seq.length (serialize st t));
+    assert (len' <= Seq.length (bare_serialize_tagged_union st tag_of_data s x));
+    assert (Seq.slice (serialize st t) 0 len' == serialize st t);
+    seq_slice_append_l (serialize st t) (serialize (s t) u);
+    assert (no_lookahead_on_precond (coerce_to_bare_parser _ pt) (serialize st t) (bare_serialize_tagged_union st tag_of_data s x));
+    assert (no_lookahead_on_postcond (coerce_to_bare_parser _ pt) (serialize st t) (bare_serialize_tagged_union st tag_of_data s x));
+    assert (Some? v1');
+    assert (injective_precond (coerce_to_bare_parser _ pt) (serialize st t) (bare_serialize_tagged_union st tag_of_data s x));
+    assert (injective_postcond (coerce_to_bare_parser _ pt) (serialize st t) (bare_serialize_tagged_union st tag_of_data s x));
+    let (Some (x1, len1)) = v1 in
+    let (Some (x1', len1')) = v1' in
+    assert (x1 == x1');
+    assert ((len1 <: nat) == (len1' <: nat));
+    assert (x1 == t);
+    assert (len1 == Seq.length (serialize st t));
+    assert (bare_serialize_tagged_union st tag_of_data s x == Seq.append (serialize st t) (serialize (s t) u));
+    seq_slice_append_r (serialize st t) (serialize (s t) u);
+    ()
+  in
+  Classical.forall_intro prf
+
+let serialize_tagged_union
+  (#tag_t: Type0)
+  (#pt: parser tag_t)
+  (st: serializer pt)
+  (#data_t: Type0)
+  (tag_of_data: (data_t -> GTot tag_t))
+  (#p: (t: tag_t) -> Tot (parser (refine_with_tag tag_of_data t)))
+  (s: (t: tag_t) -> Tot (serializer (p t)))
+: Tot (serializer (parse_tagged_union pt tag_of_data p))
+= bare_serialize_tagged_union_correct st tag_of_data s;
+  Serializer (bare_serialize_tagged_union st tag_of_data s)
